intro some abbrevs

isabelle/Distinct_Elems_Algo.thy
@@ -25,14 +25,19 @@ context
     step :: \<open>'a \<Rightarrow> 'b \<Rightarrow> 'c\<close>
 begin
 
-definition run_steps :: \<open>'e state \<Rightarrow> 'd \<Rightarrow> 'f\<close> where
-  \<open>run_steps \<equiv> flip (foldM step)\<close>
+definition run_steps :: \<open>'d \<Rightarrow> 'f\<close>  where
+  \<open>run_steps \<equiv> flip (foldM step) initial_state\<close>
 
 definition run_steps_then_estimate :: \<open>'d \<Rightarrow> 'g\<close> where
-  \<open>run_steps_then_estimate \<equiv>
-    run_steps initial_state >>> map compute_estimate\<close>
+  \<open>run_steps_then_estimate \<equiv> run_steps >>> map compute_estimate\<close>
 
 end
+
+abbreviation run_steps_pmf where
+  \<open>run_steps_pmf \<equiv> run_steps foldM_pmf\<close>
+
+abbreviation run_steps_then_estimate_pmf where
+  \<open>run_steps_then_estimate_pmf \<equiv> run_steps_then_estimate foldM_pmf map_pmf\<close>
 
 locale with_threshold =
   fixes threshold :: nat
